ironfleet/src/Dafny/Distributed/Protocol/ZooKeeper/PerformamceProof/Commons.dfy
@@ -1,0 +1,51 @@
+include "../../../Impl/Common/SeqIsUniqueDef.i.dfy"
+include "../../../Common/Framework/EnvironmentTCP.s.dfy"
+include "../Timestamps/TimestampedType.dfy"
+include "TimestampedLS.dfy"
+
+include "../Types.dfy"
+include "../DistributedSystem.dfy"
+include "../ZKEnvironment.dfy"
+include "../ZKDatabase.dfy"
+include "../Follower.dfy"
+include "../Leader.dfy"
+include "../LearnerHandler.dfy"
+include "Definitions.dfy"
+
+
+/* This module contains some common lemmas */
+module Zookeeper_Commons {
+import opened Common__SeqIsUniqueDef_i
+import opened ZKTimestamp
+import opened ZooKeeper_Types
+import opened ZooKeeper_Environment
+import opened ZooKeeper_DistributedSystem
+import opened EnvironmentTCP_s
+import opened ZooKeeper_ZKDatabase
+import opened ZooKeeper_Follower
+import opened ZooKeeper_Leader
+import opened ZooKeeper_LearnerHandler
+import opened Zookeeper_Performance_Definitions
+import opened ZooKeeper_TimestampedDistributedSystem
+
+
+predicate SentPacketsSet_Property(tls:TLS_State, tls':TLS_State, id:EndPoint, tios:seq<TZKIo>)
+    requires id in tls.t_servers;
+    requires TLS_NextOneServer(tls, tls', id, tios)
+{
+    tls'.t_environment.sentPackets == 
+    tls.t_environment.sentPackets + (set tio : TimestampedLIoOp | tio in tios && tio.LIoOpSend? :: tio.s)
+}
+
+
+lemma lemma_SentPacketsSet_Property(tls:TLS_State, tls':TLS_State, id:EndPoint, tios:seq<TZKIo>)
+    requires id in tls.t_servers;
+    requires TLS_NextOneServer(tls, tls', id, tios)
+    ensures SentPacketsSet_Property(tls, tls', id, tios)
+{
+    // TODO
+    assume false;
+}
+
+
+}
