ironfleet/src/Dafny/Distributed/Protocol/ZooKeeper/PerformamceProof/ProofEmptyDiff.dfy
@@ -13,6 +13,7 @@ include "../LearnerHandler.dfy"
 include "Definitions.dfy"
 include "PerformancePredicates.dfy"
 include "BasicInvariants.dfy"
+include "Commons.dfy"
 
 
 module Zookeeper_PerformanceProof {
@@ -30,6 +31,7 @@ import opened Zookeeper_Performance_Definitions
 import opened ZooKeeper_TimestampedDistributedSystem
 import opened Zookeeper_PerformancePredicates
 import opened Zookeeper_BasicInvariants
+import opened Zookeeper_Commons
 
 
 /* Main theorem */
@@ -85,8 +87,10 @@ predicate FollowerInfo_Message_Invariant(tls:TLS_State)
 
 lemma lemma_FollowerInfo_Message_Invariant_Induction(config:Config, tls:TLS_State, tls':TLS_State)
     requires TLS_Next(tls, tls')
-    requires Basic_Invariants(config, tls) && Basic_Invariants(config, tls')
     requires General_LS_Performance_Assumption(tls)
+    // Pre-established Invariants
+    requires Basic_Invariants(config, tls) && Basic_Invariants(config, tls')
+    requires FollowerInit_Invariant(tls);
     // Induction hypothesis
     requires FollowerInfo_Message_Invariant(tls)
     ensures FollowerInfo_Message_Invariant(tls')
@@ -95,8 +99,46 @@ lemma lemma_FollowerInfo_Message_Invariant_Induction(config:Config, tls:TLS_Stat
     var ls, ls', ios := UntagLS_State(tls), UntagLS_State(tls'), UntagLIoOpSeq(tios);
     assert LS_NextOneServer(ls, ls', actor, ios);
     if ls.servers[actor].FollowerPeer? {
-        // TODO
-        assume FollowerInfo_Message_Invariant(tls');
+        /* Here we deal with a follower taking a step */
+        var s, s' := ls.servers[actor].follower, ls'.servers[actor].follower;
+        assert FollowerNext(s, s', ios);
+        match s.state 
+        case F_HANDSHAKE_A =>  
+            assert SendMyInfo(s, s', ios);
+            assert tls.t_servers[actor].ts == TimeZero();  // by FollowerInit_Invariant
+            assert |ios| == |tios| == 1;
+            var tio : TimestampedLIoOp := tios[0];
+            assert tio.LIoOpSend?;
+            var hs := ActionToHostStep(tls, tls', actor, tios);
+            assert tls'.t_servers[actor].ts == TLS_NoRecvPerfUpdate(tls.t_servers[actor].ts, hs);
+            assert tio.s.msg.ts == SendFI;
+            lemma_SentPacketsSet_Property(tls, tls', actor, tios);
+        case F_HANDSHAKE_B => 
+            assert AcceptNewEpoch(s, s', ios);
+            assert ios[0].LIoOpReceive?;
+            if ios[0].r.msg.newZxid.epoch < s.accepted_epoch {
+                assert |ios| == 1;
+                assert forall io | io in ios :: !io.LIoOpSend?;
+            } else { 
+                assert |ios| == 2;
+                assert ios[1].LIoOpSend?;
+                assert ios[1].s.msg.AckEpoch?;
+                assert !ios[1].s.msg.FollowerInfo?;
+                forall i | 0 <= i < |ios| 
+                ensures ios[i].LIoOpSend? ==> ios[i].s.msg.AckEpoch? {
+                    if i == 0 {
+                        assert ios[i].LIoOpReceive?;
+                    } else {
+                        assert i == 1;
+                        assert ios[i].LIoOpSend? && ios[i].s.msg.AckEpoch?;
+                    }
+                }
+            }
+        case F_SYNC => 
+            assert SyncWithLeader(s, s', ios);
+            assert forall io | io in ios && io.LIoOpSend? :: !io.s.msg.FollowerInfo?;
+        case F_RUNNING => assert |ios| == 0;       
+        case F_ERROR => assert |ios| == 0;
     } else {
         /* No new FollowerInfo messages get sent, so nothing to worry */
         var s, s' := ls.servers[actor].leader, ls'.servers[actor].leader;
